isabelle-thys/Basic_Rules.thy
@@ -36,7 +36,8 @@ lemma substitution1_function_index_flip: "substitution1_function (index_flip_sub
 
 lemma index_flip_var_raw_substitution1_footprint: "index_flip_var_raw ` substitution1_footprint s =
   substitution1_footprint (index_flip_substitute1 s)"
-  sorry
+  apply (cases "Rep_substitution1 s")
+  by (simp add: substitution1_footprint.rep_eq index_flip_substitute1.rep_eq)
 
 lemma index_flip_substitute1_twice[simp]: "index_flip_substitute1 (index_flip_substitute1 s) = s"
   apply transfer by (auto simp: image_iff)
@@ -194,6 +195,36 @@ lemma bi_unique_rel_expression[transfer_rule]:
 lemma rel_substitute1_flip[simp]: "(rel_substitute1 R S)^--1 = rel_substitute1 R^--1 S^--1"
   apply (rule ext)+ unfolding conversep_iff apply transfer by auto
 
+lemma rel_substitute1x_flip[simp]: "(rel_substitute1x R S)^--1 = rel_substitute1x R^--1 S^--1"
+  apply (rule ext)+ unfolding rel_substitute1x_def by (auto simp: rel_fun_def simp flip: rel_mem2_flip)
+
+lemma left_unique_rel_substitute1x[transfer_rule]: 
+  assumes "left_unique R"
+  assumes "left_unique S"
+    and "right_total S"
+    and "type_preserving_var_rel S"
+  shows "left_unique (rel_substitute1x R S)"
+proof (unfold rel_substitute1x_def, rule left_uniqueI, auto)
+  fix x y z
+  assume "R (substitution1_variable x) (substitution1_variable z)"
+    and "R (substitution1_variable y) (substitution1_variable z)"
+  with \<open>left_unique R\<close> have "substitution1_variable x = substitution1_variable y"
+    by (rule left_uniqueD)
+  moreover
+  assume "rel_set R (substitution1_footprint x) (substitution1_footprint z)"
+    and "rel_set R (substitution1_footprint y) (substitution1_footprint z)"
+  with \<open>left_unique R\<close> have "substitution1_footprint x = substitution1_footprint y"
+    by (meson left_uniqueD left_unique_rel_set)
+  moreover
+  assume "rel_fun (rel_mem2 S) (=) (substitution1_function x) (substitution1_function z)"
+    and "rel_fun (rel_mem2 S) (=) (substitution1_function y) (substitution1_function z)"
+  with assms have "substitution1_function x = substitution1_function y"
+    by (meson left_total_rel_mem2 left_uniqueD left_unique_eq left_unique_fun)
+  ultimately
+  show "x = y"
+    using Rep_substitution1_components Rep_substitution1_inject by auto
+qed
+
 lemma left_unique_rel_substitute1[transfer_rule]: 
   assumes "left_unique R"
   assumes "left_unique S"
@@ -263,10 +294,103 @@ lemma right_unique_rel_substitute1[transfer_rule]:
   apply (rule left_unique_rel_substitute1)
   using assms by auto
 
+lemma right_unique_rel_substitute1x[transfer_rule]:
+  assumes "right_unique R" and "right_unique S" and "left_total S" and "type_preserving_var_rel S"
+  shows "right_unique (rel_substitute1x R S)"
+  apply (subst conversep_conversep[of R, symmetric])
+  apply (subst conversep_conversep[of S, symmetric])
+  apply (subst rel_substitute1x_flip[symmetric])
+  apply (simp del: rel_substitute1x_flip)
+  apply (rule left_unique_rel_substitute1x)
+  using assms by auto
+
 lemma bi_unique_rel_substitute1[transfer_rule]:
   assumes "bi_unique R" and "bi_unique S"
   shows "bi_unique (rel_substitute1 R S)"
   using assms by (meson bi_total_alt_def bi_unique_alt_def left_unique_rel_substitute1 right_unique_rel_substitute1)
+
+lemma bi_unique_rel_substitute1x[transfer_rule]:
+  assumes "bi_unique R" and "bi_unique S" and "bi_total S" and "type_preserving_var_rel S"
+  shows "bi_unique (rel_substitute1x R S)"
+  using assms by (meson bi_total_alt_def bi_unique_alt_def left_unique_rel_substitute1x right_unique_rel_substitute1x)
+
+lemma rel_set_subst_expression_footprint_x:
+  includes lifting_syntax
+  assumes "bi_unique R" and "bi_total R" and "type_preserving_var_rel R"  (* TODO cleanup *)
+  defines "subR == rel_substitute1x R R" (* TODO must be (=) ? *)
+  assumes "list_all2 subR s1 s2"
+  assumes "rel_set R vs1 vs2" 
+  shows "rel_set R (subst_expression_footprint s1 vs1) (subst_expression_footprint s2 vs2)"
+proof (rule rel_setI)
+
+  have goal: "\<exists>y\<in>subst_expression_footprint s2 vs2. R x y" if "x \<in> subst_expression_footprint s1 vs1" 
+    and [transfer_rule]: "list_all2 subR s1 s2"
+    and [transfer_rule]: "rel_set R vs1 vs2"
+    and [transfer_rule]: "bi_unique R"
+    and [transfer_rule]: "bi_total R"
+    and [transfer_rule]: "type_preserving_var_rel R"
+    and subR_def: "subR = rel_substitute1x R R"
+  for x s1 s2 vs1 vs2 R subR
+  proof -
+    have [transfer_rule]: "(subR ===> R) substitution1_variable substitution1_variable"
+      unfolding subR_def by (rule rel_substitute1x_substitution1_variable)
+    have [transfer_rule]: "(subR ===> rel_set R) substitution1_footprint substitution1_footprint"
+      unfolding subR_def by (rule rel_substitute1x_substitution1_footprint)
+    have [transfer_rule]: "bi_unique subR" 
+      unfolding subR_def
+      using \<open>bi_unique R\<close> apply (rule bi_unique_rel_substitute1x)
+      using that bi_unique_eq by auto
+    show ?thesis
+    proof (cases "x \<in> vs1 - substitution1_variable ` set s1")
+      case False
+      with that obtain sx vx where x_sx: "x \<in> substitution1_footprint sx" 
+        and Some1: "Some sx = find (\<lambda>s. substitution1_variable s = vx) s1" 
+        and sx_vs1: "substitution1_variable sx \<in> vs1"
+        unfolding subst_expression_footprint_def by auto
+      from Some1 obtain i where s1i: "s1!i = sx" and lens1: "i < length s1"
+        by (metis find_Some_iff) 
+      define sy where "sy = s2!i"
+      then have [transfer_rule]: "subR sx sy" (* and "i < length s2" *)
+        using s1i lens1 \<open>list_all2 subR s1 s2\<close> list_all2_conv_all_nth by blast
+      from Some1 have vx_def: "vx = substitution1_variable sx"
+        by (metis (mono_tags) find_Some_iff)
+      define vy where "vy = substitution1_variable sy"
+      have [transfer_rule]: "R vx vy" unfolding vy_def vx_def
+        by (meson \<open>(subR ===> R) substitution1_variable substitution1_variable\<close> \<open>subR sx sy\<close> rel_funD)
+      from sx_vs1 have "vx : vs1"
+        by (simp add: vx_def)
+      have Some2: "Some sy = find (\<lambda>s. substitution1_variable s = vy) s2"
+        apply (transfer fixing: sy vy s1) 
+        by (fact Some1)
+      have sy_vs2: "substitution1_variable sy \<in> vs2"
+        apply (transfer fixing: sy vs2)
+        by (fact sx_vs1)
+      have "rel_set R (substitution1_footprint sx) (substitution1_footprint sy)"
+        by (meson \<open>(subR ===> rel_set R) substitution1_footprint substitution1_footprint\<close> \<open>subR sx sy\<close> rel_funD)
+      with x_sx obtain y where Rxy: "R x y" and y_sy: "y \<in> substitution1_footprint sy"
+        by (meson rel_set_def)
+      from Some2 sy_vs2 y_sy have "y\<in>subst_expression_footprint s2 vs2"
+        unfolding subst_expression_footprint_def by auto
+      with Rxy show ?thesis by auto
+    next
+      case True
+      have "rel_set R (vs1 - substitution1_variable ` set s1) (vs2 - substitution1_variable ` set s2)"
+        by transfer_prover
+      with True obtain y where "y \<in> vs2 - substitution1_variable ` set s2" and Rxy: "R x y"
+        by (meson rel_set_def)
+      then have "y\<in>subst_expression_footprint s2 vs2"
+        unfolding subst_expression_footprint_def by auto
+      with Rxy show ?thesis by auto 
+    qed
+  qed
+  show "\<exists>y\<in>subst_expression_footprint s2 vs2. R x y" if "x \<in> subst_expression_footprint s1 vs1" for x
+    apply (rule goal) using assms that by simp_all
+  show "\<exists>x\<in>subst_expression_footprint s1 vs1. R x y" if "y \<in> subst_expression_footprint s2 vs2" for y
+    apply (subst conversep_iff[of R, symmetric])
+    apply (rule goal[where R="conversep R" and subR="conversep subR"]) 
+          apply (simp_all add: list.rel_flip)
+    using that assms by (simp_all add: subR_def)
+qed
 
 lemma rel_set_subst_expression_footprint:
   includes lifting_syntax
@@ -347,6 +471,14 @@ proof (rule rel_setI)
     using that assms by (simp_all add: subR_def)
 qed
 
+lemma rel_substitution1x_function:
+  includes lifting_syntax
+  fixes R S
+  defines "subR == rel_substitute1x R S"
+  shows "(subR ===> rel_mem2 S ===> (=)) substitution1_function substitution1_function"
+  unfolding subR_def rel_substitute1x_def apply (rule rel_funI)+ unfolding rel_fun_def
+  apply transfer by auto
+
 lemma rel_substitution1_function:
   includes lifting_syntax
   fixes R
@@ -361,6 +493,64 @@ proof (rule rel_funI, rule rel_funI, rename_tac s1 s2 m1 m2)
     apply transfer unfolding rel_fun_def rel_set_def apply auto
     by (meson inv_into_injective range_subsetD)
 qed
+
+lemma rel_subst_mem2_x:
+  includes lifting_syntax
+  fixes R
+  assumes [transfer_rule]: "bi_unique R"
+  defines "subR == rel_substitute1x R R"
+  shows "(list_all2 subR ===> rel_mem2 R ===> rel_mem2 R) subst_mem2 subst_mem2"
+proof (rule rel_funI, rule rel_funI)
+  fix s1 s2 m1 m2
+  assume s12[unfolded subR_def, transfer_rule]: "list_all2 subR s1 s2"
+  assume m12[transfer_rule]: "rel_mem2 R m1 m2"
+  show "rel_mem2 R (subst_mem2 s1 m1) (subst_mem2 s2 m2)"
+    unfolding rel_mem2.rep_eq subst_mem2.rep_eq 
+  proof (rule rel_funI, rename_tac v1 v2) 
+    fix v1 v2
+    assume v12[transfer_rule]: "R v1 v2"
+    note rel_substitute1x_substitution1_variable[transfer_rule]
+    define find1 find2 
+      where "find1 = find (\<lambda>s. substitution1_variable s = v1) s1" 
+        and "find2 = find (\<lambda>s. substitution1_variable s = v2) s2"
+    have find12: "(rel_option subR) find1 find2" 
+      unfolding find1_def find2_def subR_def
+      by transfer_prover
+    show "(case find1 of None \<Rightarrow> Rep_mem2 m1 v1 | Some s \<Rightarrow> substitution1_function s m1) =
+          (case find2 of None \<Rightarrow> Rep_mem2 m2 v2 | Some s \<Rightarrow> substitution1_function s m2)"
+    proof (cases "find1")
+      case None
+      with find12 have None2: "find2 = None" by auto
+      show ?thesis
+        unfolding None None2 apply simp
+        by (metis (full_types) v12 m12 rel_fun_def rel_mem2.rep_eq)
+    next
+      case (Some s1')
+      with find12 obtain s2' where Some2: "find2 = Some s2'" and [transfer_rule]: "subR s1' s2'"
+        by (meson option_rel_Some1)
+      have [transfer_rule]: "(subR ===> rel_mem2 R ===> (=)) substitution1_function substitution1_function"
+         unfolding subR_def by (rule rel_substitution1x_function)
+      show ?thesis
+        unfolding Some Some2 apply simp by transfer_prover
+    qed
+  qed
+qed
+(*   apply (rule rel_funI)+ unfolding subR_def
+  apply transfer
+  apply auto
+  
+  (* using rel_mem2.transfer[transfer_rule] apply (tactic \<open>all_tac\<close>) *)
+             apply (unfold Transfer.Rel_def)[1]
+             apply (rule rel_mem2.transfer)
+  using rel_mem2.transfer
+  find_theorems rel_mem2 name:trans
+  apply transfer_step
+  apply transfer_step
+  apply transfer_step
+  apply transfer_step
+  apply transfer_step
+  apply transfer_step
+  apply transfer_step *)
 
 lemma rel_subst_mem2:
   includes lifting_syntax
@@ -401,6 +591,7 @@ proof (rule rel_funI, rule rel_funI)
     qed
   qed
 qed
+
 
 lemma rel_expression_subst_expression [transfer_rule]: 
   includes lifting_syntax
@@ -450,6 +641,54 @@ proof -
     apply (rule_tac rel_funI)+ by assumption
 qed
 
+lemma rel_expression_subst_expression_x [transfer_rule]: 
+  includes lifting_syntax
+  assumes [transfer_rule]: "bi_unique R" and [transfer_rule]: "bi_total R" and [transfer_rule]: "type_preserving_var_rel R" (* TODO cleanup *)
+  defines "subR == rel_substitute1x R R" (* TODO different R/S? *)
+  shows "(list_all2 subR ===> rel_expression R (=) ===> rel_expression R (=)) 
+         subst_expression subst_expression"
+proof -
+  have "rel_expression R (=) (subst_expression s1 e1) (subst_expression s2 e2)" 
+    if subR_s1_s2[transfer_rule]: "list_all2 subR s1 s2" and R_e1_e2: "rel_expression R (=) e1 e2" 
+    for s1 s2 and e1 e2 :: "'b expression"
+  proof -
+    define vs1 E1 vs2 E2 where "vs1 = expression_vars e1" and "E1 = expression_eval e1"
+      and "vs2 = expression_vars e2" and "E2 = expression_eval e2"
+    have [unfolded subR_def, transfer_rule]: 
+      "(subR ===> rel_prod R (rel_prod (rel_set R) (rel_mem2 R ===> (=)))) Rep_substitution1 Rep_substitution1"
+      unfolding subR_def by (rule rel_substitute1x_Rep_substitution1)
+    have [transfer_rule]: "(subR ===> R) substitution1_variable substitution1_variable"
+      unfolding subR_def by (rule rel_substitute1x_substitution1_variable)
+    have [transfer_rule]: "bi_unique subR" 
+      unfolding subR_def
+      using \<open>bi_unique R\<close> apply (rule bi_unique_rel_substitute1x)
+      by (auto simp: assms)
+    have [transfer_rule]: "(subR ===> rel_set R) substitution1_footprint substitution1_footprint"
+      unfolding subR_def by (rule rel_substitute1x_substitution1_footprint)
+    have R_vs1_vs2[transfer_rule]: "rel_set R vs1 vs2"
+      unfolding vs1_def vs2_def using R_e1_e2 apply transfer by auto
+    have foot: "rel_set R (subst_expression_footprint s1 vs1) (subst_expression_footprint s2 vs2)"
+      apply (rule rel_set_subst_expression_footprint_x)
+      using assms R_vs1_vs2 subR_s1_s2 unfolding subR_def by auto
+    have E1E2: "(rel_mem2 R ===> (=)) E1 E2" 
+      unfolding E1_def E2_def apply (rule rel_funI)
+      using R_e1_e2 apply transfer 
+      unfolding rel_mem2.rep_eq rel_fun_def by auto
+    have subst_mem2_s1_s2: "(rel_mem2 R ===> rel_mem2 R) (subst_mem2 s1) (subst_mem2 s2)"
+      using rel_subst_mem2_x subR_s1_s2 \<open>bi_unique R\<close>
+      by (metis rel_fun_def subR_def)
+    from E1E2 subst_mem2_s1_s2 have subst: "(rel_mem2 R ===> (=)) (E1 \<circ> subst_mem2 s1) (E2 \<circ> subst_mem2 s2)"
+      by (smt comp_def rel_funD rel_funI)
+    show ?thesis
+      unfolding rel_expression.rep_eq subst_expression.rep_eq using foot subst
+      by (simp add: Rep_expression_components E1_def E2_def vs1_def vs2_def)
+  qed
+
+  then show ?thesis
+     unfolding subR_def
+    apply (rule_tac rel_funI)+ by assumption
+qed
+
 definition "rel_flip_index x y \<longleftrightarrow> index_flip_var_raw x = y"
 lemma rel_flip_index_def': "rel_flip_index x y \<longleftrightarrow> x = index_flip_var_raw y"
     unfolding rel_flip_index_def by auto
@@ -471,7 +710,7 @@ lemma rel_flip_index_conversep[simp]: "rel_flip_index\<inverse>\<inverse> = rel_
   apply (rule ext)+ unfolding conversep_iff using rel_flip_index_def rel_flip_index_def' by auto
 
 lemma index_flip_subst_expression: 
-  fixes \<sigma> :: "substitution1 list" and e :: "'a::universe expression"
+  fixes \<sigma> :: "substitution1 list" and e :: "'a expression"
   shows "index_flip_expression (subst_expression \<sigma> e) 
         = subst_expression (map index_flip_substitute1 \<sigma>) (index_flip_expression e)"
 proof -
@@ -523,8 +762,9 @@ proof -
 
   have "rel_substitute1x rel_flip_index rel_flip_index s (index_flip_substitute1 s)" (* if "niceS s" *) for s
     unfolding rel_substitute1x_def  
-    using Fx by (auto simp: rel_flip_index_def substitution1_variable_index_flip substitution1_function_index_flip rel_fun_def)
-
+    using Fx
+    by (metis (mono_tags, lifting) index_flip_var_raw_substitution1_footprint rel_flip_index_def rel_funI rel_set_rel_flip_index substitution1_function_index_flip substitution1_variable_index_flip)
+  
   then have index_flip_substitute1_transfer [transfer_rule]:
     "((=) ===> subR) (%x. x) index_flip_substitute1"
     unfolding subR_def rel_fun_def by auto
@@ -537,19 +777,14 @@ proof -
 
   have [transfer_rule]: "(list_all2 subR ===> rel_expression rel_flip_index (=) ===> rel_expression rel_flip_index (=))
    subst_expression subst_expression"
-    unfolding subR_def by transfer_prover
+    unfolding subR_def
+    by transfer_prover
 
   have "(rel_expression (=) (=))
         (index_flip_expression (subst_expression \<sigma> e))
         (id (subst_expression (map index_flip_substitute1 \<sigma>) (index_flip_expression e)))"
     apply transfer_prover_start
-           apply transfer_step
-           apply transfer_step
-           apply transfer_step
-           apply transfer_step
-           apply transfer_step
-           apply transfer_step
-           apply transfer_step
+           apply transfer_step+
     by simp
   then
   show "index_flip_expression (subst_expression \<sigma> e) = subst_expression (map index_flip_substitute1 \<sigma>) (index_flip_expression e)"
@@ -557,13 +792,13 @@ proof -
 qed
 
 
-(* TODO move *)
+(* (* TODO move *)
 lemma index_flip_subst_expression: 
   fixes \<sigma> :: "substitution1 list" and e :: "'a::universe expression"
   shows "index_flip_expression (subst_expression \<sigma> e) 
         = subst_expression (map index_flip_substitute1 \<sigma>) (index_flip_expression e)"
 proof -
-  define subR where "subR = (rel_substitute1 rel_flip_index (rel_expression rel_flip_index ((=)::'a\<Rightarrow>'a\<Rightarrow>bool)))" 
+  define subR where "subR = rel_substitute1x rel_flip_index rel_flip_index" 
   
   have rel_set_rel_flip_index: "rel_set rel_flip_index x y \<longleftrightarrow> index_flip_var_raw ` x = y" for x y
     unfolding rel_set_def rel_flip_index_def by auto
@@ -601,22 +836,26 @@ proof -
   then have inv_embedding_index_flip_mem2: "(rel_mem2 rel_flip_index ===> (=)) (inv embedding \<circ> f) (inv embedding \<circ> (f \<circ> index_flip_mem2))" for f
     apply (rule_tac rel_funI) by simp
 
-  have 1: "rel_prod rel_flip_index (\<lambda>(vs1, f1) (vs2, f2). 
+(*   have 1: "rel_prod rel_flip_index (\<lambda>(vs1, f1) (vs2, f2). 
               rel_prod (rel_set rel_flip_index) (rel_mem2 rel_flip_index ===> (=)) 
                        (vs1, inv embedding \<circ> f1) (vs2, inv embedding \<circ> f2))
               (v, vs, f) (index_flip_var_raw v, index_flip_var_raw ` vs, f \<circ> index_flip_mem2)" for v vs f
-    by (auto intro: rel_flip_index_index_flip_var_raw rel_set_rel_flip_index_index_flip_var_raw inv_embedding_index_flip_mem2)
+    by (auto intro: rel_flip_index_index_flip_var_raw rel_set_rel_flip_index_index_flip_var_raw inv_embedding_index_flip_mem2) *)
 
-  define niceS where "niceS s \<longleftrightarrow> variable_raw_domain (substitution1_variable s) = range (embedding::'a\<Rightarrow>_)" for s
-  define niceR where "niceR s1 s2 \<longleftrightarrow> s1=s2 \<and> niceS s1" for s1 s2
+  (* define niceS where "niceS s \<longleftrightarrow> variable_raw_domain (substitution1_variable s) = range (embedding::'a\<Rightarrow>_)" for s *)
+  (* define niceR where "niceR s1 s2 \<longleftrightarrow> s1=s2 \<and> niceS s1" for s1 s2 *)
 
-  have "rel_substitute1 rel_flip_index (rel_expression rel_flip_index ((=)::'a\<Rightarrow>_\<Rightarrow>_)) s (index_flip_substitute1 s)" if "niceS s" for s
-    using [[show_types, show_consts]]
-    using that[unfolded niceS_def]
-    apply transfer apply (case_tac s) using 1 by auto
+  have "rel_substitute1x rel_flip_index rel_flip_index s (index_flip_substitute1 s)" (* if "niceS s" *) for s
+    unfolding rel_substitute1x_def apply auto
+    apply (metis rel_flip_index_index_flip_var_raw substitution1_variable_index_flip)
+    apply (metis index_flip_var_raw_substitution1_footprint rel_set_rel_flip_index_index_flip_var_raw)
+    (* using [[show_types, show_consts]] *)
+    (* using that[unfolded niceS_def] *)
+    (* apply transfer apply (case_tac s) using 1 by auto *)
+    by x
   then have index_flip_substitute1_transfer [transfer_rule]: 
-    "(niceR ===> subR) (%x. x) index_flip_substitute1"
-    unfolding niceR_def subR_def rel_fun_def by auto
+    "((=) ===> subR) (%x. x) index_flip_substitute1"
+    unfolding (* niceR_def *) subR_def rel_fun_def by auto
 (*   have [transfer_rule]: "bi_unique (rel_expression rel_flip_index (=))"
     sorry *)
   have "index_flip_expression e = f" if that[transfer_rule]: "rel_expression rel_flip_index (=) e f" for e f :: "'c expression"
@@ -632,20 +871,12 @@ proof -
         (index_flip_expression (subst_expression \<sigma> e))
         (id (subst_expression (map index_flip_substitute1 \<sigma>) (index_flip_expression e)))"
     apply transfer_prover_start
-           apply transfer_step
-           apply transfer_step
-           apply transfer_step
-           apply transfer_step
-           apply transfer_step
-           apply transfer_step
-           apply transfer_step
-           apply transfer_step
-    find_theorems map name:transfer
+           apply transfer_step+
     by simp
   then
   show "index_flip_expression (subst_expression \<sigma> e) = subst_expression (map index_flip_substitute1 \<sigma>) (index_flip_expression e)"
     unfolding rel_expression_eq id_def by assumption
-qed
+qed *)
 
 (* (* TODO move *)
 lemma index_flip_subst_expression: "index_flip_expression (subst_expression \<sigma> e) 
@@ -832,7 +1063,7 @@ lemma assign2_rule:
   shows "qrhl A [] [assign x e] B"
   using [[simproc del: index_var]]
   apply (rule sym_rule)
-  apply (simp add: assms index_flip_subst_expression index_flip_substitute1 index_flip_var_index_var index_flip_expression_index_expression)
+  apply (simp add: assms index_flip_subst_expression index_flip_substitute1 index_flip_expression_index_expression)
   by (rule assign1_rule)
 
 lemma sample1_rule:
